RelationalAlgebra/Equivalence/RAtoFOL/Rename.lean
@@ -3,9 +3,9 @@ import RelationalAlgebra.Equivalence.RAtoFOL.Conversion
 variable {dbi f q} [struc : FOL.folStruc dbi]
 
 theorem ra_to_fol_evalT.r_def.mp (h : RA.Query.isWellTyped dbi.schema (.r f q))
-  (ih: ∀t, (ra_to_fol_query q dbi.schema).RealizeDom dbi t → t ∈ RA.Query.evaluateT dbi q) :
-    ∀t, (ra_to_fol_query (.r f q) dbi.schema).RealizeDom dbi t → t ∈ RA.Query.evaluateT dbi (.r f q) := by
-      simp only [RA.Query.isWellTyped.r_def, ra_to_fol_query, FOL.Query.RealizeDom.def,
+  (ih: ∀t, (ra_to_fol_query q dbi.schema).RealizeMin dbi t → t ∈ RA.Query.evaluateT dbi q) :
+    ∀t, (ra_to_fol_query (.r f q) dbi.schema).RealizeMin dbi t → t ∈ RA.Query.evaluateT dbi (.r f q) := by
+      simp only [RA.Query.isWellTyped.r_def, ra_to_fol_query, FOL.Query.RealizeMin.def,
         FOL.BoundedQuery.Realize.relabel_def, Nat.add_zero, Fin.castAdd_zero, Fin.cast_refl,
         CompTriple.comp_eq, Fin.natAdd_zero, FOL.BoundedQuery.relabel_schema, Function.comp_apply,
         Sum.getLeft?_inl, Part.coe_some, Finset.pimage_some, Finset.coe_image,
@@ -22,14 +22,14 @@ theorem ra_to_fol_evalT.r_def.mp (h : RA.Query.isWellTyped dbi.schema (.r f q))
           simp_all [right.1 hx'']
 
 theorem ra_to_fol_evalT.r_def.mpr (h : RA.Query.isWellTyped dbi.schema (.r f q))
-  (ih : ∀t ∈ RA.Query.evaluateT dbi q, (ra_to_fol_query q dbi.schema).RealizeDom dbi t) :
-    ∀t, t ∈ RA.Query.evaluateT dbi (.r f q) → (ra_to_fol_query (.r f q) dbi.schema).RealizeDom dbi t := by
+  (ih : ∀t ∈ RA.Query.evaluateT dbi q, (ra_to_fol_query q dbi.schema).RealizeMin dbi t) :
+    ∀t, t ∈ RA.Query.evaluateT dbi (.r f q) → (ra_to_fol_query (.r f q) dbi.schema).RealizeMin dbi t := by
       intro t h_RA_eval
       apply And.intro ?_
         (by simp_all [RA.Query.evaluate.validSchema (.r f q) h t h_RA_eval, ra_to_fol_query_schema])
 
       simp only [ra_to_fol_query]
-      simp_all only [FOL.Query.RealizeDom.def, ra_to_fol_query.isWellTyped, ra_to_fol_query_schema,
+      simp_all only [FOL.Query.RealizeMin.def, ra_to_fol_query.isWellTyped, ra_to_fol_query_schema,
         RA.Query.isWellTyped.r_def, RA.Query.evaluateT.r_def, renameT, exists_eq_right',
         Set.mem_setOf_eq, forall_const, and_self, implies_true]
       obtain ⟨left, right⟩ := h
