RelationalAlgebra/Equivalence/RAtoFOL/Selection.lean
@@ -3,15 +3,15 @@ import RelationalAlgebra.Equivalence.RAtoFOL.Conversion
 variable {dbi a b p q} [struc : FOL.folStruc dbi]
 
 theorem ra_to_fol_evalT.s_def.mp (h : RA.Query.isWellTyped dbi.schema (.s a b p q))
-  (ih: ∀t, (ra_to_fol_query q dbi.schema).RealizeDom dbi t → t ∈ RA.Query.evaluateT dbi q) :
-    ∀t, (ra_to_fol_query (.s a b p q) dbi.schema).RealizeDom dbi t → t ∈ RA.Query.evaluateT dbi (.s a b p q) := by
+  (ih: ∀t, (ra_to_fol_query q dbi.schema).RealizeMin dbi t → t ∈ RA.Query.evaluateT dbi q) :
+    ∀t, (ra_to_fol_query (.s a b p q) dbi.schema).RealizeMin dbi t → t ∈ RA.Query.evaluateT dbi (.s a b p q) := by
       intro t
       simp only [RA.Query.isWellTyped.s_def, ra_to_fol_query, FOL.outVar.def,
-        FOL.Query.RealizeDom.def, FOL.BoundedQuery.Realize.def, FOL.BoundedQuery.toFormula_tEq,
+        FOL.Query.RealizeMin.def, FOL.BoundedQuery.Realize.def, FOL.BoundedQuery.toFormula_tEq,
         FirstOrder.Language.BoundedFormula.realize_inf, FOL.BoundedQuery.schema.tEq_def,
         RA.Query.evaluateT.s_def, selectionT, ↓reduceIte, Set.mem_setOf_eq, and_imp] at ⊢ h
       intro a_1 a_2 a_3
-      simp_all only [FOL.Query.RealizeDom.def, ra_to_fol_query.isWellTyped, and_imp]
+      simp_all only [FOL.Query.RealizeMin.def, ra_to_fol_query.isWellTyped, and_imp]
       obtain ⟨left, right⟩ := h
       obtain ⟨left_1, right⟩ := right
       apply And.intro
@@ -21,14 +21,14 @@ theorem ra_to_fol_evalT.s_def.mp (h : RA.Query.isWellTyped dbi.schema (.s a b p 
       · exact a_2
 
 theorem ra_to_fol_evalT.s_def.mpr (h : RA.Query.isWellTyped dbi.schema (.s a b p q))
-  (ih : ∀t ∈ RA.Query.evaluateT dbi q, (ra_to_fol_query q dbi.schema).RealizeDom dbi t) :
-    ∀t, t ∈ RA.Query.evaluateT dbi (.s a b p q) → (ra_to_fol_query (.s a b p q) dbi.schema).RealizeDom dbi t := by
+  (ih : ∀t ∈ RA.Query.evaluateT dbi q, (ra_to_fol_query q dbi.schema).RealizeMin dbi t) :
+    ∀t, t ∈ RA.Query.evaluateT dbi (.s a b p q) → (ra_to_fol_query (.s a b p q) dbi.schema).RealizeMin dbi t := by
       intro t h_RA_eval
       apply And.intro ?_
         (by simp_all [RA.Query.evaluate.validSchema (.s a b p q) h t h_RA_eval, ra_to_fol_query_schema])
 
       simp only [ra_to_fol_query]
-      simp_all only [RA.Query.isWellTyped.s_def, FOL.Query.RealizeDom.def,
+      simp_all only [RA.Query.isWellTyped.s_def, FOL.Query.RealizeMin.def,
         FOL.BoundedQuery.Realize.def, ra_to_fol_query_schema, RA.Query.evaluateT.s_def, selectionT,
         ne_eq, ite_true, Set.mem_setOf_eq, FOL.outVar.def, FOL.BoundedQuery.toFormula_tEq,
         FirstOrder.Language.BoundedFormula.realize_inf, true_and]
